% The entire content of this work (including the source code
% for TeX files and the generated PDF documents) by 
% Hongxiang Chen (nicknamed we.taper, or just Taper) is
% licensed under a 
% Creative Commons Attribution-NonCommercial-ShareAlike 4.0 
% International License (Link to the complete license text:
% http://creativecommons.org/licenses/by-nc-sa/4.0/).
\documentclass{article}

% My own physics package
% The following line load the package xparse with additional option to
% prevent the annoying warnings, which are caused by the package
% "physics" loaded in package "physicist-taper".
\usepackage[log-declarations=false]{xparse}
\usepackage{physicist-taper}

\title{Solution for HW6 20161109}
\date{\today}
\author{Taper}

\begin{document}

\maketitle
\abstract{
\begin{CJK}{UTF8}{gbsn}陈鸿翔（11310075）\end{CJK}
}
%\tableofcontents
\section{Validate that \texorpdfstring{$\Tr=\sum \lambda_i$ with
$\sigma_x$}{}}
The characteristic equations is
\begin{align*}
    &\det \left( \begin{array}{cc}
        -\lambda & 1 \\
        1 & -\lambda \\
    \end{array} \right) = 0 \\
    &\Rightarrow \lambda^2 -1 = 0 \\
    &\Rightarrow \lambda = \pm 1 \\
    &\Rightarrow \lambda_1 + \lambda_2 = 0
\end{align*}
Meanwhile, we have $\Tr(\sigma_x) = 0+0 = 0$, confirming theorem.

\section{Prove \texorpdfstring{$[X,Y]=[Y,Z]=[X,Z]=0$}{}}
% \int \dd x\ket{x}\bra{x} x
% \int \dd y\ket{y}\bra{y} y
% \int \dd z\ket{z}\bra{z} z
\begin{align*}
    [X,Y] &= \int \dd x\ket{x}\bra{x} x \int \dd y\ket{y}\bra{y} y
        - \int \dd y\ket{y}\bra{y} y \int \dd x\ket{x}\bra{x} x \\
        &= \iint \dx\dy (xy - yx) \ket{x}\bra{x}\ket{y}\bra{y} \\
        &= \iint \dx\dy \, 0 \ket{x}\bra{x}\ket{y}\bra{y} \\
        &= 0
\end{align*}
Similarly,

\begin{align*}
    [Y,Z] &= \int \dd y\ket{y}\bra{y} y \int \dd z\ket{z}\bra{z} z
        - \int \dd z\ket{z}\bra{z} z \int \dd y\ket{y}\bra{y} y \\
        &= \iint \dy\dz (yz - zy) \ket{y}\bra{y}\ket{z}\bra{z} \\
        &= \iint \dy\dz \, 0 \ket{y}\bra{y}\ket{z}\bra{z} \\
        &= 0
\end{align*}


\begin{align*}
    [X,Z] &= \int \dd x\ket{x}\bra{x} x \int \dd z\ket{z}\bra{z} z
        - \int \dd z\ket{z}\bra{z} z \int \dd x\ket{x}\bra{x} x \\
        &= \iint \dx\dz (xz - zx) \ket{x}\bra{x}\ket{z}\bra{z} \\
        &= \iint \dx\dz \, 0 \ket{x}\bra{x}\ket{z}\bra{z} \\
        &= 0
\end{align*}

\section{Prove}
\subsection{Translation operator is unitary}
\begin{proof}
Since
\begin{align*}
    \ket{T_a \beta} \equiv T_a \ket{\beta} &= T_a \int \dd[3]{x}
    \ket{x} \braket{x|\beta} \\
        &=  \int \dd[3]{x} \ket{x+b} \braket{x|\beta}
\end{align*}
So
\begin{align*}
    \bra{T_a \beta} = \int \dd[3]{x} \braket{x|\beta}^* \bra{x+b}
\end{align*}
Then 
\begin{align*}
    \braket{T_a \beta|\gamma } &= \int \dd[3]{x} \braket{x|\beta}^* \bra{x+b}
        \int \dd[3]{x'} \braket{x'|\gamma} \ket{x'}\\
        &= \iint\dd[3]{x}\dd[3]{x'}\delta(x+a-x')
        \braket{x|\beta}^*\braket{x'|\gamma} \\
        &= \iint\dd[3]{x}\dd[3]{x'}\delta(x-(x'-a))
        \braket{x|\beta}^*\braket{x'|\gamma} \\
        &= \int \dd[3]{x} \braket{x|\beta}^* \bra{x}
        \int \dd[3]{x'} \braket{x'|\gamma} \ket{x'-a}\\
        &= \int \dd[3]{x} \braket{x|\beta}^* \bra{x}
        \left(T_{-a} \int \dd[3]{x'} \braket{x'|\gamma} \ket{x'}\right)\\
        &= \braket{\beta | T_{-a} \gamma}
\end{align*}
So
\begin{equation}
    T_a^\dagger = T_{-a}
\end{equation}
So, with the result of section~\ref{sec:3.3}, we have
\begin{align*}
    T_a T_a^\dagger = T_a T_{-a} = T_{a-a} = T_0 = \id
\end{align*}
\end{proof}
Hence it is unitary.
\subsection{\texorpdfstring{$[T_a,T_b]=0$}{}}
\begin{proof}
Notice that
\begin{align*}
    T_{a+b} \ket{\alpha} = T_{a+b} \int \dd[3]{x} \ket{x} \braket{x|\alpha}
    &=  \int \dd[3]{x} \ket{x+(a+b)} \braket{x|\alpha} \\
    &=  \int \dd[3]{x} \ket{x+(b+a)} \braket{x|\alpha} \\
    &=  T_{b+a} \int \dd[3]{x} \ket{x} \braket{x|\alpha} \\
    &=  T_{b+a} \ket{\alpha}
\end{align*}
So $T_{a+b} = T_{b+a}$. Then use the result of section \ref{sec:3.3},
we have
\begin{align*}
    [T_a,T_b] = T_a T_b - T_b T_a = T_{a+b} - T_{b+a} = T_{a+b} -
    T_{a+b} = 0
\end{align*}
\end{proof}

\subsection{\texorpdfstring{$T_a T_b = T_{a+b}$}{}}
\label{sec:3.3}
\begin{proof}
\begin{align*}
    T_a T_b \ket{\alpha} &= T_a T_b \int \dd[3]{x} \ket{x}
        \braket{x|\alpha} \\
        &=  T_a \int \dd[3]{x} \ket{x+b} \braket{x|\alpha} \\
        &=  \int \dd[3]{x} \ket{x+b+a} \braket{x|\alpha} \\
        &=  \int \dd[3]{x} \ket{x+(a+b)} \braket{x|\alpha} \\
        &=  T_{a+b} \int \dd[3]{x} \ket{x} \braket{x|\alpha}
\end{align*}
So $T_a T_b = T_{a+b}$.
\end{proof}

\end{document}
